Repair and progress on correct termination

Simple_Clause_Learning/Correct_Termination.thy
@@ -4,7 +4,7 @@ begin
 
 context scl begin
 
-lemma assumes "(regular_scl N)\<^sup>*\<^sup>* initial_state S" and "conflict N S S'"
+(* lemma assumes "(regular_scl N \<beta>)\<^sup>*\<^sup>* initial_state S" and "conflict N \<beta> S S'"
   shows "\<exists>C \<gamma>. state_conflict S' = Some (C, \<gamma>) \<and>
     (trail_level_cls (state_trail S) (C \<cdot> \<gamma>) = trail_level (state_trail S))"
   using \<open>conflict N S S'\<close>
@@ -97,15 +97,6 @@ lemma
 proof -  
   oops
 
-lemma not_satisfiable_if_sound_state_conflict_bottom:
-  assumes sound_S: "sound_state N S" and conflict_S: "state_conflict S = Some ({#}, \<gamma>)"
-  shows "\<not> satisfiable (grounding_of_clss N)"
-proof -
-  from sound_S conflict_S have "N \<TTurnstile>\<G>e {{#}}"
-    unfolding sound_state_def state_conflict_def by auto
-  thus ?thesis by simp
-qed
-
 lemma
   assumes sound: "sound_state N (\<Gamma>, U, Some (C' + {#L#}, \<gamma>))"
   shows
@@ -173,14 +164,439 @@ lemma trail_interp_clss_if_sound_and_trail_true:
   shows "trail_interp \<Gamma> \<TTurnstile>s CC"
   using \<open>trail_true_clss \<Gamma> CC\<close> trail_interp_cls_if_sound_and_trail_true[OF \<open>sound_trail N U \<Gamma>\<close>]
   by (simp add: trail_true_clss_def true_clss_def)
+ *)
+
+lemma not_satisfiable_if_sound_state_conflict_bottom:
+  assumes sound_S: "sound_state N S" and conflict_S: "state_conflict S = Some ({#}, \<gamma>)"
+  shows "\<not> satisfiable (grounding_of_clss N)"
+proof -
+  from sound_S conflict_S have "N \<TTurnstile>\<G>e {{#}}"
+    unfolding sound_state_def state_conflict_def by auto
+  thus ?thesis by simp
+qed
+
+definition adapt_subst_to_renaming where
+  "adapt_subst_to_renaming \<rho> \<sigma> x =
+    (if x \<in> the_Var ` \<rho> ` subst_domain \<sigma> then
+      \<sigma> (the_inv \<rho> (Var x))
+    else
+      Var x)"
+
+lemma subst_lit_renaming_subst_adapted:
+  assumes ren_\<rho>: "is_renaming \<rho>" and vars_L: "vars_lit L \<subseteq> subst_domain \<sigma>"
+  shows "L \<cdot>l \<rho> \<cdot>l adapt_subst_to_renaming \<rho> \<sigma> = L \<cdot>l \<sigma>"
+  unfolding subst_lit_comp_subst[symmetric]
+proof (intro same_on_vars_lit ballI)
+  fix x assume "x \<in> vars_lit L"
+  with vars_L have x_in: "x \<in> subst_domain \<sigma>"
+    by blast
+
+  obtain x' where \<rho>_x: "\<rho> x = Var x'"
+    using ren_\<rho>[unfolded is_renaming_iff]
+    by (meson is_Var_def)
+  with x_in have x'_in: "x' \<in> the_Var ` \<rho> ` subst_domain \<sigma>"
+    by (metis image_eqI term.sel(1))
+
+  have "(\<rho> \<odot> adapt_subst_to_renaming \<rho> \<sigma>) x = \<rho> x \<cdot>a adapt_subst_to_renaming \<rho> \<sigma>"
+    by (simp add: subst_compose_def)
+  also have "... = adapt_subst_to_renaming \<rho> \<sigma> x'"
+    using \<rho>_x by simp
+  also have "... = \<sigma> (the_inv \<rho> (Var x'))"
+    by (simp add: adapt_subst_to_renaming_def if_P[OF x'_in])
+  also have "... = \<sigma> (the_inv \<rho> (\<rho> x))"
+    by (simp add: \<rho>_x)
+  also have "... = \<sigma> x"
+    using ren_\<rho>[unfolded is_renaming_iff]
+    by (simp add: the_inv_f_f)
+  finally show "(\<rho> \<odot> adapt_subst_to_renaming \<rho> \<sigma>) x = \<sigma> x"
+    by simp
+qed
+
+lemma subst_renaming_subst_adapted:
+  assumes ren_\<rho>: "is_renaming \<rho>" and vars_D: "vars_cls D \<subseteq> subst_domain \<sigma>"
+  shows "D \<cdot> \<rho> \<cdot> adapt_subst_to_renaming \<rho> \<sigma> = D \<cdot> \<sigma>"
+  unfolding subst_cls_comp_subst[symmetric]
+proof (intro same_on_lits_clause ballI)
+  fix L assume "L \<in># D"
+  with vars_D have "vars_lit L \<subseteq> subst_domain \<sigma>"
+    by (auto dest!: multi_member_split)
+  thus "L \<cdot>l (\<rho> \<odot> adapt_subst_to_renaming \<rho> \<sigma>) = L \<cdot>l \<sigma>"
+    unfolding subst_lit_comp_subst
+    by (rule subst_lit_renaming_subst_adapted[OF ren_\<rho>])
+qed
+
+lemma vars_cls_subset_subst_domain_if_grounding:
+  assumes "is_ground_cls (C \<cdot> \<sigma>)"
+  shows "vars_cls C \<subseteq> subst_domain \<sigma>"
+proof (rule Set.subsetI)
+  fix x assume "x \<in> vars_cls C"
+  thus "x \<in> subst_domain \<sigma>"
+    unfolding subst_domain_def mem_Collect_eq
+    by (metis assms empty_iff is_ground_atm_iff_vars_empty is_ground_cls_is_ground_on_var
+        term.set_intros(3))
+qed
+
+lemma vars_lit_subst_subset_vars_cls_substI[intro]:
+  "vars_lit L \<subseteq> vars_cls C \<Longrightarrow> vars_lit (L \<cdot>l \<sigma>) \<subseteq> vars_cls (C \<cdot> \<sigma>)"
+  by (metis subset_Un_eq subst_cls_add_mset vars_cls_add_mset vars_subst_cls_eq)
+
+lemma ball_image_mset: "(\<forall>x \<in># image_mset f M. P x) \<longleftrightarrow> (\<forall>x \<in># M. P (f x))"
+  by blast
+
+lemma ball_filter_mset: "(\<forall>x \<in># filter_mset P M. Q x) \<longleftrightarrow> (\<forall>x \<in># M. P x \<longrightarrow> Q x)"
+  by fastforce
+
+lemma set_list_of_mset[simp]: "set (list_of_mset M) = set_mset M"
+  by (rule set_mset_mset[of "list_of_mset _", unfolded mset_list_of_mset, symmetric])
+
+lemma ex_unify_if_unifiers_not_empty:
+  "unifiers es \<noteq> {} \<Longrightarrow> set xs = es \<Longrightarrow> \<exists>ys. unify xs [] = Some ys"
+  using unify_complete by auto
+
+lemma not_empty_if_mem: "x \<in> X \<Longrightarrow> X \<noteq> {}"
+  by blast
+
+lemma propagate_if_conflict_follows_decide:
+  assumes
+    fin_N: "finite N" and fin_learned: "finite (state_learned S\<^sub>0)" and
+    no_conf: "\<nexists>S\<^sub>1. conflict N \<beta> S\<^sub>0 S\<^sub>1" and deci: "decide N \<beta> S\<^sub>0 S\<^sub>2" and conf: "conflict N \<beta> S\<^sub>2 S\<^sub>3"
+  shows "\<exists>S\<^sub>4. propagate N \<beta> S\<^sub>0 S\<^sub>4"
+proof -
+  from deci obtain L \<gamma> \<Gamma> U where
+    S\<^sub>0_def: "S\<^sub>0 = (\<Gamma>, U, None)" and
+    S\<^sub>2_def: "S\<^sub>2 = (trail_decide \<Gamma> (L \<cdot>l \<gamma>), U, None)" and
+    "L \<in> \<Union> (set_mset ` N)" and
+    "is_ground_lit (L \<cdot>l \<gamma>)" and
+    "\<not> trail_defined_lit \<Gamma> (L \<cdot>l \<gamma>)"
+    by (elim decide.cases) blast
+  with conf obtain D D' \<sigma> where
+    S\<^sub>3_def: "S\<^sub>3 = (trail_decide \<Gamma> (L \<cdot>l \<gamma>), U, Some (D', \<sigma>))" and
+    D_in: "D \<in> N \<union> U" and
+    D'_def: "D' = rename_clause (N \<union> U \<union> clss_of_trail (trail_decide \<Gamma> (L \<cdot>l \<gamma>))) D" and
+    "subst_domain \<sigma> \<subseteq> vars_cls D'" and
+    ground_D'_\<sigma>: "is_ground_cls (D' \<cdot> \<sigma>)" and
+    tr_\<Gamma>_L_false_D': "trail_false_cls (trail_decide \<Gamma> (L \<cdot>l \<gamma>)) (D' \<cdot> \<sigma>)"
+    by (elim conflict.cases) blast
+
+  define \<rho> :: "'v \<Rightarrow> ('f, 'v) Term.term" where
+    "\<rho> = renaming_wrt (N \<union> U \<union> clss_of_trail \<Gamma>)"
+
+  have ren_\<rho>: "is_renaming \<rho>"
+    unfolding \<rho>_def
+    by (metis S\<^sub>0_def fin_N fin_learned finite_UnI finite_clss_of_trail is_renaming_renaming_wrt
+        state_learned_simp)
+
+  have is_renaming_wrt_N_U_\<Gamma>_L: "is_renaming (renaming_wrt (N \<union> U \<union> clss_of_trail (trail_decide \<Gamma> (L \<cdot>l \<gamma>))))"
+    by (metis S\<^sub>0_def fin_N fin_learned finite_UnI finite_clss_of_trail is_renaming_renaming_wrt
+        state_learned_simp)
+
+  from D_in D'_def ground_D'_\<sigma> tr_\<Gamma>_L_false_D' obtain \<sigma>' where
+    "is_ground_cls (D \<cdot> \<sigma>')" and "trail_false_cls ((L \<cdot>l \<gamma>, None) # \<Gamma>) (D \<cdot> \<sigma>')"
+    unfolding trail_decide_def by (metis rename_clause_def subst_cls_comp_subst)
+  moreover have
+    nex_false_grounding: "\<nexists>\<sigma>. is_ground_cls (D \<cdot> \<sigma>) \<and> trail_false_cls \<Gamma> (D \<cdot> \<sigma>)"
+    unfolding not_ex de_Morgan_conj
+  proof (rule allI)
+    fix \<delta>
+    from no_conf[simplified, rule_format, of \<Gamma> U "Some (D', restrict_subst (vars_cls D')
+      (adapt_subst_to_renaming (renaming_wrt (N \<union> U \<union> clss_of_trail (trail_decide \<Gamma> (L \<cdot>l \<gamma>))))
+        (restrict_subst (vars_cls D) \<delta>)))"]
+    show "\<not> is_ground_cls (D \<cdot> \<delta>) \<or> \<not> trail_false_cls \<Gamma> (D \<cdot> \<delta>)"
+      apply (simp add: D'_def rename_clause_def conflict.simps S\<^sub>0_def subst_cls_restrict_subst_idem subst_domain_restrict_subst)
+      using subst_renaming_subst_adapted[OF is_renaming_wrt_N_U_\<Gamma>_L, of D "restrict_subst (vars_cls D) \<delta>"]
+      by (smt (verit) D'_def S\<^sub>0_def S\<^sub>3_def
+          \<open>\<And>thesis. (\<And>D D' \<sigma>. \<lbrakk>S\<^sub>3 = (trail_decide \<Gamma> (L \<cdot>l \<gamma>), U, Some (D', \<sigma>)); D \<in> N \<union> U; D' = rename_clause (N \<union> U \<union> clss_of_trail (trail_decide \<Gamma> (L \<cdot>l \<gamma>))) D; subst_domain \<sigma> \<subseteq> vars_cls D'; is_ground_cls (D' \<cdot> \<sigma>); trail_false_cls (trail_decide \<Gamma> (L \<cdot>l \<gamma>)) (D' \<cdot> \<sigma>)\<rbrakk> \<Longrightarrow> thesis) \<Longrightarrow> thesis\<close>
+          \<open>\<not> conflict N \<beta> S\<^sub>0 (\<Gamma>, U, Some (D', restrict_subst (vars_cls D') (adapt_subst_to_renaming (renaming_wrt (N \<union> U \<union> clss_of_trail (trail_decide \<Gamma> (L \<cdot>l \<gamma>)))) (restrict_subst (vars_cls D) \<delta>))))\<close>
+          clss_of_trail_trail_decide conflict.intros equalityD1 option.inject prod.simps(1)
+          rename_clause_def vars_cls_subset_subst_domain_if_grounding subst_cls_restrict_subst_idem
+          subst_domain_restrict_subst)
+  qed
+  ultimately have "- (L \<cdot>l \<gamma>) \<in># D \<cdot> \<sigma>'"
+    using subtrail_falseI by blast
+  then obtain D'' L' where D_def: "D = add_mset L' D''" and "- (L \<cdot>l \<gamma>) = L' \<cdot>l \<sigma>'"
+    by (meson Melem_subst_cls multi_member_split)
+
+  have 1: "D'' \<cdot> \<rho> + {#L' \<cdot>l \<rho>#} = rename_clause (N \<union> U \<union> clss_of_trail \<Gamma>) D"
+    unfolding D_def rename_clause_def
+    by (simp add: \<rho>_def)
+
+  have "inj \<rho>"
+    unfolding \<rho>_def
+    apply (rule inj_Var_renaming)
+    using fin_N fin_learned
+    by (simp add: S\<^sub>0_def)
+
+  define \<sigma>'' where
+    "\<sigma>'' = adapt_subst_to_renaming \<rho> \<sigma>'"
+
+  define \<sigma>''' where
+    "\<sigma>''' = restrict_subst (vars_cls (D'' \<cdot> \<rho>) \<union> vars_lit (L' \<cdot>l \<rho>)) \<sigma>''"
+
+  have 2: "subst_domain \<sigma>''' \<subseteq> vars_cls (D'' \<cdot> \<rho>) \<union> vars_lit (L' \<cdot>l \<rho>)"
+    by (simp add: \<sigma>'''_def subst_domain_restrict_subst)
+
+  have "D \<cdot> \<sigma>' = D \<cdot> \<rho> \<cdot> \<sigma>''"
+    unfolding \<sigma>''_def
+  proof (rule subst_renaming_subst_adapted[symmetric])
+    show "is_renaming \<rho>"
+      unfolding \<rho>_def
+      by (metis S\<^sub>0_def fin_N fin_learned finite_UnI finite_clss_of_trail is_renaming_renaming_wrt
+          state_learned_simp)
+  next
+    show "vars_cls D \<subseteq> subst_domain \<sigma>'"
+      using \<open>is_ground_cls (D \<cdot> \<sigma>')\<close>
+      by (auto intro!: vars_cls_subset_subst_domain_if_grounding)
+  qed
+  hence "D \<cdot> \<sigma>' = D \<cdot> \<rho> \<cdot> \<sigma>'''"
+    unfolding \<sigma>'''_def
+    by (metis "1" \<rho>_def rename_clause_def subst_cls_restrict_subst_idem sup_bot.right_neutral
+        sup_ge1 vars_cls_add_mset vars_cls_empty vars_cls_plus_iff)
+  hence 3: "is_ground_cls ((D'' \<cdot> \<rho> + {#L' \<cdot>l \<rho>#}) \<cdot> \<sigma>''')"
+    using 1[unfolded rename_clause_def, folded \<rho>_def, symmetric]
+    using \<open>is_ground_cls (D \<cdot> \<sigma>')\<close>
+    by presburger
+
+  have not_false_if_grounding:
+    "is_ground_cls (add_mset (L' \<cdot>l \<rho>) (D'' \<cdot> \<rho>) \<cdot> \<sigma>) \<Longrightarrow>
+      \<not> trail_false_cls \<Gamma> (add_mset (L' \<cdot>l \<rho>) (D'' \<cdot> \<rho>) \<cdot> \<sigma>)" for \<sigma>
+    using nex_false_grounding[simplified, rule_format, of "\<rho> \<odot> _", simplified]
+    unfolding 1[unfolded rename_clause_def, folded \<rho>_def, symmetric]
+    by simp
+
+  have "L' \<cdot>l \<rho> \<cdot>l \<sigma>''' = L' \<cdot>l \<rho> \<cdot>l \<sigma>''"
+    unfolding \<sigma>'''_def
+    by (meson inf_sup_ord(4) subst_lit_restrict_subst_idem)
+
+  have "D'' \<cdot> \<rho> \<cdot> \<sigma>''' = D'' \<cdot> \<rho> \<cdot> \<sigma>''"
+    unfolding \<sigma>'''_def
+    by (meson inf_sup_ord subst_cls_restrict_subst_idem)
+
+  have "{#K \<in># D'' \<cdot> \<rho>. K \<cdot>l \<sigma>''' \<noteq> L' \<cdot>l \<rho> \<cdot>l \<sigma>'''#} =
+    {#K \<in># D''. K \<cdot>l \<rho> \<cdot>l \<sigma>''' \<noteq> L' \<cdot>l \<rho> \<cdot>l \<sigma>'''#} \<cdot> \<rho>"
+    unfolding subst_cls_def[of D'']
+    unfolding image_mset_filter_mset_swap[symmetric]
+    unfolding subst_cls_def[symmetric]
+    by (rule refl)
+
+  have "{#K \<in># D''. K \<cdot>l \<rho> \<cdot>l \<sigma>''' \<noteq> L' \<cdot>l \<rho> \<cdot>l \<sigma>''#} =
+    {#K \<in># D''. K \<cdot>l \<rho> \<cdot>l \<sigma>'' \<noteq> L' \<cdot>l \<rho> \<cdot>l \<sigma>''#}"
+  proof (rule filter_mset_cong0)
+    fix K assume "K \<in># D''"
+    hence "vars_lit K \<subseteq> vars_cls D''"
+      using multi_member_split by fastforce
+    hence "vars_lit (K \<cdot>l \<rho>) \<subseteq> vars_cls (D'' \<cdot> \<rho>)"
+      by (rule vars_lit_subst_subset_vars_cls_substI)
+    hence *: "vars_lit (K \<cdot>l \<rho>) \<subseteq> vars_cls (D'' \<cdot> \<rho>) \<union> vars_lit (L' \<cdot>l \<rho>)"
+      by blast
+
+    show "(K \<cdot>l \<rho> \<cdot>l \<sigma>''' \<noteq> L' \<cdot>l \<rho> \<cdot>l \<sigma>'') = (K \<cdot>l \<rho> \<cdot>l \<sigma>'' \<noteq> L' \<cdot>l \<rho> \<cdot>l \<sigma>'')"
+      unfolding \<sigma>'''_def
+      unfolding subst_lit_restrict_subst_idem[OF *]
+      by (rule refl)
+  qed
+
+  have "{#K \<in># D'' \<cdot> \<rho>. K \<cdot>l \<sigma>''' \<noteq> L' \<cdot>l \<rho> \<cdot>l \<sigma>'''#} \<cdot> \<sigma>''' =
+    {#K \<in># D''. K \<cdot>l \<rho> \<cdot>l \<sigma>'' \<noteq> L' \<cdot>l \<rho> \<cdot>l \<sigma>''#} \<cdot> \<rho> \<cdot> \<sigma>''"
+    unfolding \<open>{#K \<in># D'' \<cdot> \<rho>. K \<cdot>l \<sigma>''' \<noteq> L' \<cdot>l \<rho> \<cdot>l \<sigma>'''#} = {#K \<in># D''. K \<cdot>l \<rho> \<cdot>l \<sigma>''' \<noteq> L' \<cdot>l \<rho> \<cdot>l \<sigma>'''#} \<cdot> \<rho>\<close>
+    unfolding \<open>L' \<cdot>l \<rho> \<cdot>l \<sigma>''' = L' \<cdot>l \<rho> \<cdot>l \<sigma>''\<close>
+    unfolding \<open>{#K \<in># D''. K \<cdot>l \<rho> \<cdot>l \<sigma>''' \<noteq> L' \<cdot>l \<rho> \<cdot>l \<sigma>''#} = {#K \<in># D''. K \<cdot>l \<rho> \<cdot>l \<sigma>'' \<noteq> L' \<cdot>l \<rho> \<cdot>l \<sigma>''#}\<close>
+    unfolding \<sigma>'''_def
+  proof (rule subst_cls_restrict_subst_idem)
+    have "vars_cls ({#K \<in># D''. K \<cdot>l \<rho> \<cdot>l \<sigma>'' \<noteq> L' \<cdot>l \<rho> \<cdot>l \<sigma>''#} \<cdot> \<rho>) \<subseteq> vars_cls (D'' \<cdot> \<rho>)"
+      by (metis multiset_filter_subset subset_mset.le_iff_add subst_cls_mono_mset sup_ge1
+          vars_cls_plus_iff)
+    thus "vars_cls ({#K \<in># D''. K \<cdot>l \<rho> \<cdot>l \<sigma>'' \<noteq> L' \<cdot>l \<rho> \<cdot>l \<sigma>''#} \<cdot> \<rho>) \<subseteq> vars_cls (D'' \<cdot> \<rho>) \<union>
+      vars_lit (L' \<cdot>l \<rho>) "
+      by fast
+  qed
+
+  have "vars_cls D \<subseteq> subst_domain \<sigma>'"
+    by (rule \<open>is_ground_cls (D \<cdot> \<sigma>')\<close>[THEN vars_cls_subset_subst_domain_if_grounding])
+
+  have "vars_cls D'' \<subseteq> subst_domain \<sigma>'" "vars_lit L' \<subseteq> subst_domain \<sigma>'"
+    using \<open>is_ground_cls (D \<cdot> \<sigma>')\<close>[THEN vars_cls_subset_subst_domain_if_grounding]
+    unfolding D_def
+    by simp_all
+
+  have "{#K \<in># D''. K \<cdot>l \<rho> \<cdot>l \<sigma>'' \<noteq> L' \<cdot>l \<sigma>'#} \<subseteq># D''"
+    by simp
+  hence "vars_cls {#K \<in># D''. K \<cdot>l \<rho> \<cdot>l \<sigma>'' \<noteq> L' \<cdot>l \<sigma>'#} \<subseteq> vars_cls D''"
+    by (metis multiset_partition sup_ge1 vars_cls_plus_iff)
+  with \<open>vars_cls D'' \<subseteq> subst_domain \<sigma>'\<close> have
+    "vars_cls {#K \<in># D''. K \<cdot>l \<rho> \<cdot>l \<sigma>'' \<noteq> L' \<cdot>l \<sigma>'#} \<subseteq> subst_domain \<sigma>'"
+    by fast
+
+  have 4: "trail_false_cls \<Gamma> ({#K \<in># D'' \<cdot> \<rho>. K \<cdot>l \<sigma>''' \<noteq> L' \<cdot>l \<rho> \<cdot>l \<sigma>'''#} \<cdot> \<sigma>''')"
+    using \<open>trail_false_cls ((L \<cdot>l \<gamma>, None) # \<Gamma>) (D \<cdot> \<sigma>')\<close>[
+        unfolded \<open>D \<cdot> \<sigma>' = D \<cdot> \<rho> \<cdot> \<sigma>'''\<close> 1[unfolded rename_clause_def, folded \<rho>_def, symmetric],
+        simplified]
+    using not_false_if_grounding[of \<sigma>''', simplified, OF 3[simplified]]
+    unfolding \<open>{#K \<in># D'' \<cdot> \<rho>. K \<cdot>l \<sigma>''' \<noteq> L' \<cdot>l \<rho> \<cdot>l \<sigma>'''#} \<cdot> \<sigma>''' =
+       {#K \<in># D''. K \<cdot>l \<rho> \<cdot>l \<sigma>''  \<noteq> L' \<cdot>l \<rho> \<cdot>l \<sigma>''#} \<cdot> \<rho> \<cdot> \<sigma>''\<close>
+    unfolding \<open>L' \<cdot>l \<rho> \<cdot>l \<sigma>''' = L' \<cdot>l \<rho> \<cdot>l \<sigma>''\<close> \<open>D'' \<cdot> \<rho> \<cdot> \<sigma>''' = D'' \<cdot> \<rho> \<cdot> \<sigma>''\<close>
+    unfolding subst_lit_renaming_subst_adapted[OF ren_\<rho> \<open>vars_lit L' \<subseteq> subst_domain \<sigma>'\<close>, folded \<sigma>''_def]
+    unfolding subst_renaming_subst_adapted[OF ren_\<rho> \<open>vars_cls D'' \<subseteq> subst_domain \<sigma>'\<close>, folded \<sigma>''_def]
+    unfolding subst_renaming_subst_adapted[OF ren_\<rho>
+        \<open>vars_cls {#K \<in># D''. K \<cdot>l \<rho> \<cdot>l \<sigma>'' \<noteq> L' \<cdot>l \<sigma>'#} \<subseteq> subst_domain \<sigma>'\<close>, folded \<sigma>''_def]
+    unfolding \<open>- (L \<cdot>l \<gamma>) = L' \<cdot>l \<sigma>'\<close>[symmetric]
+    unfolding trail_false_cls_def trail_false_lit_def list.set image_insert prod.sel
+    unfolding subst_cls_def ball_image_mset ball_filter_mset
+    by (smt (verit, ccfv_threshold) \<open>vars_cls D'' \<subseteq> subst_domain \<sigma>'\<close> \<rho>_def \<sigma>''_def
+        add_mset_add_single clss_of_trail_trail_decide image_insert insert_DiffM insert_iff
+        is_renaming_wrt_N_U_\<Gamma>_L le_sup_iff mk_disjoint_insert multiset.set_map
+        subst_lit_renaming_subst_adapted uminus_lit_swap union_iff vars_cls_add_mset)
+
+  have 5: "\<not> trail_defined_lit \<Gamma> (L' \<cdot>l \<rho> \<cdot>l \<sigma>''')"
+    unfolding \<open>L' \<cdot>l \<rho> \<cdot>l \<sigma>''' = L' \<cdot>l \<rho> \<cdot>l \<sigma>''\<close>
+    unfolding subst_lit_renaming_subst_adapted[OF ren_\<rho> \<open>vars_lit L' \<subseteq> subst_domain \<sigma>'\<close>, folded \<sigma>''_def]
+    unfolding \<open>- (L \<cdot>l \<gamma>) = L' \<cdot>l \<sigma>'\<close>[symmetric]
+    using \<open>\<not> trail_defined_lit \<Gamma> (L \<cdot>l \<gamma>)\<close>
+    by (metis trail_defined_lit_iff_defined_uminus)
+
+  let ?xs =
+    "map atm_of (list_of_mset (add_mset (L' \<cdot>l \<rho>) {#K \<in># D'' \<cdot> \<rho>. K \<cdot>l \<sigma>''' = L' \<cdot>l \<rho> \<cdot>l \<sigma>'''#}))"
+
+  have "unifiers (set (pairs ?xs)) \<noteq> {}"
+  proof (rule not_empty_if_mem)
+    show "\<sigma>''' \<in> unifiers (set (pairs ?xs))"
+      unfolding subst_cls_def[of D'']
+      unfolding image_mset_filter_mset_swap[symmetric]
+      unfolding subst_cls_def[symmetric]
+      unfolding unifiers_def mem_Collect_eq
+      unfolding set_pairs list.set_map set_list_of_mset
+      unfolding split_paired_Ball_Sigma prod.sel
+      unfolding set_mset_add_mset_insert image_insert
+      unfolding subst_cls_def set_image_mset set_mset_filter
+      by (smt (verit, ccfv_SIG) image_iff insert_iff mem_Collect_eq subst_atm_of_eqI)
+  qed
+
+  then obtain ys where
+    unify_pairs: "unify (pairs ?xs) [] = Some ys"
+    using ex_unify_if_unifiers_not_empty[OF _ refl]
+    by blast
+
+  define \<mu> where
+    "\<mu> = subst_of ys"
+
+  have 6: "is_mimgu \<mu>
+    {atm_of ` set_mset (add_mset (L' \<cdot>l \<rho>) {#K \<in># D'' \<cdot> \<rho>. K \<cdot>l \<sigma>''' = L' \<cdot>l \<rho> \<cdot>l \<sigma>'''#})}"
+  proof (intro is_mimgu_if_mgu_sets[unfolded mgu_sets_def] exI conjI)
+    show "set (map set [?xs]) = {atm_of ` set_mset
+      (add_mset (L' \<cdot>l \<rho>) {#K \<in># D'' \<cdot> \<rho>. K \<cdot>l \<sigma>''' = L' \<cdot>l \<rho> \<cdot>l \<sigma>'''#})}"
+      by simp
+  next
+    show "map_option subst_of (unify (concat (map pairs
+      [map atm_of (list_of_mset (add_mset (L' \<cdot>l \<rho>) {#K \<in># D'' \<cdot> \<rho>. K \<cdot>l \<sigma>''' = L' \<cdot>l \<rho> \<cdot>l \<sigma>'''#}))]))
+      []) = Some \<mu>"
+      by (simp add: unify_pairs \<mu>_def)
+  qed
+
+  have 7: "\<forall>K\<in>#add_mset (L' \<cdot>l \<rho>) (D'' \<cdot> \<rho>) \<cdot> \<sigma>'''. K \<prec>\<^sub>B \<beta>"
+    sorry
+
+  show ?thesis
+    using propagateI[OF D_in 1 2 3 refl refl 4 5 6 refl 7]
+    unfolding S\<^sub>0_def by blast
+qed
+
+lemma ex_mgu_if_subst_eq_subst:
+  assumes "t \<cdot>a \<sigma> = u \<cdot>a \<sigma>"
+  shows "\<exists>\<mu>. Unification.mgu t u = Some \<mu>"
+proof -
+  from assms have "unifiers {(t, u)} \<noteq> {}"
+    unfolding unifiers_def by auto
+  then obtain xs where unify: "unify [(t, u)] [] = Some xs"
+    using ex_unify_if_unifiers_not_empty[of "{(t, u)}" "[(t, u)]"]
+    by auto
+
+  show ?thesis
+  proof (rule exI)
+    show "Unification.mgu t u = Some (subst_of xs)"
+      using unify
+      by (simp add: Unification.mgu.simps)
+  qed
+qed
+
+lemma range_vars_eq_empty_if_is_ground:
+  "is_ground_cls (C \<cdot> \<gamma>) \<Longrightarrow> subst_domain \<gamma> \<subseteq> vars_cls C \<Longrightarrow> range_vars \<gamma> = {}"
+  unfolding range_vars_def UNION_empty_conv subst_range.simps is_ground_cls_iff_vars_empty
+  by (metis (no_types, opaque_lifting) dual_order.eq_iff imageE is_ground_atm_iff_vars_empty
+      is_ground_cls_iff_vars_empty is_ground_cls_is_ground_on_var
+      vars_cls_subset_subst_domain_if_grounding)
+
+definition trail_propagated_wf where
+  "trail_propagated_wf \<Gamma> \<longleftrightarrow> (\<forall>(L\<^sub>\<gamma>, n) \<in> set \<Gamma>.
+    case n of
+      None \<Rightarrow> True
+    | Some (_, L, \<gamma>) \<Rightarrow> L\<^sub>\<gamma> = L \<cdot>l \<gamma>)"
+
+lemma "sound_trail N U \<Gamma> \<Longrightarrow> trail_propagated_wf \<Gamma>"
+proof (induction \<Gamma> rule: sound_trail.induct)
+  case Nil
+  then show ?case
+    by (simp add: trail_propagated_wf_def)
+next
+  case (Cons \<Gamma> L u)
+  then show ?case
+    by (cases u) (auto simp add: trail_propagated_wf_def)
+qed
+
+definition trail_minimal_subst_domains where
+  "trail_minimal_subst_domains \<Gamma> \<longleftrightarrow> (\<forall>(_, n) \<in> set \<Gamma>.
+    case n of
+      None \<Rightarrow> True
+    | Some (C, L, \<gamma>) \<Rightarrow> subst_domain \<gamma> \<subseteq> vars_cls (add_mset L C))"
+
+lemma "sound_trail N U \<Gamma> \<Longrightarrow> trail_minimal_subst_domains \<Gamma>"
+proof (induction \<Gamma> rule: sound_trail.induct)
+  case Nil
+  then show ?case
+    by (simp add: trail_minimal_subst_domains_def)
+next
+  case (Cons \<Gamma> L u)
+  then show ?case
+    by (cases u) (auto simp add: trail_minimal_subst_domains_def)
+qed
+
+definition trail_groundings where
+  "trail_groundings \<Gamma> \<longleftrightarrow> (\<forall>(_, n) \<in> set \<Gamma>.
+    case n of
+      None \<Rightarrow> True
+    | Some (C, L, \<gamma>) \<Rightarrow> is_ground_cls (add_mset L C \<cdot> \<gamma>))"
+
+lemma "sound_trail N U \<Gamma> \<Longrightarrow> trail_groundings \<Gamma>"
+proof (induction \<Gamma> rule: sound_trail.induct)
+  case Nil
+  then show ?case
+    by (simp add: trail_groundings_def)
+next
+  case (Cons \<Gamma> L u)
+  then show ?case
+    by (cases u) (auto simp add: trail_groundings_def)
+qed
+
+definition conflict_grounding where
+  "conflict_grounding u \<longleftrightarrow> (case u of None \<Rightarrow> True | Some (C, \<gamma>) \<Rightarrow> is_ground_cls (C \<cdot> \<gamma>))"
+
+lemma "sound_state N S \<Longrightarrow> conflict_grounding (state_conflict S)"
+  by (cases "state_conflict S") (auto simp add: sound_state_def conflict_grounding_def)
+
+definition conflict_minimal_subst_domain where
+  "conflict_minimal_subst_domain u \<longleftrightarrow> (case u of None \<Rightarrow> True | Some (C, \<gamma>) \<Rightarrow> subst_domain \<gamma> \<subseteq> vars_cls C)"
 
 lemma
   assumes
-    fin_N: "finite N" and disj_N: "disjoint_vars_set N" and
-    regular_run: "(regular_scl N)\<^sup>*\<^sup>* initial_state S" and
-    no_more_regular_step: "\<nexists>S'. regular_scl N S S'"
+    fin_N: "finite N" and fin_learned_S: "finite (state_learned S)" and
+    disj_N: "disjoint_vars_set N" and
+    trail_propagate_wf: "trail_propagated_wf (state_trail S)" and
+    trail_min_subst_dom: "trail_minimal_subst_domains (state_trail S)" and
+    trail_groundings: "trail_groundings (state_trail S)" and
+    conflict_min_subst_dom: "conflict_minimal_subst_domain (state_conflict S)" and
+    regular_run: "(regular_scl N \<beta>)\<^sup>*\<^sup>* initial_state S" and
+    no_more_regular_step: "\<nexists>S'. regular_scl N \<beta> S S'"
   shows "\<not> satisfiable (grounding_of_clss N) \<and> (\<exists>\<gamma>. state_conflict S = Some ({#}, \<gamma>)) \<or>
-  (\<exists>\<gamma>. trail_true_clss (state_trail S) (N \<cdot>cs \<gamma>))"
+    satisfiable {C \<in> grounding_of_clss N. multp (\<prec>\<^sub>B) C {#\<beta>#}} \<and>
+      trail_true_clss (state_trail S) {C \<in> grounding_of_clss N. multp (\<prec>\<^sub>B) C {#\<beta>#}}"
 proof -
   obtain \<Gamma> U u where S_def: "S = (\<Gamma>, U, u)"
     using prod_cases3 by blast
@@ -188,14 +604,14 @@ proof -
   have sound_S: "sound_state N S"
     using regular_run_sound_state[OF regular_run] sound_initial_state[OF fin_N disj_N] by blast
 
-  from no_more_regular_step have no_new_conflict: "\<nexists>S'. conflict N S S'"
+  from no_more_regular_step have no_new_conflict: "\<nexists>S'. conflict N \<beta> S S'"
     using regular_scl_def by blast
 
-  from no_more_regular_step have no_propagate: "\<nexists>S'. propagate N S S'"
+  from no_more_regular_step have no_new_propagate: "\<nexists>S'. propagate N \<beta> S S'"
     by (meson decide_well_defined(1) local.scl_def reasonable_scl_def regular_scl_def)
 
   from no_more_regular_step have
-    no_reasonable_decide: "(\<nexists>S'. decide N S S') \<or> (\<exists>S' S''. decide N S S' \<and> conflict N S' S'')"
+    no_reasonable_decide: "(\<nexists>S'. decide N \<beta> S S') \<or> (\<exists>S' S''. decide N \<beta> S S' \<and> conflict N \<beta> S' S'')"
     using local.scl_def reasonable_scl_def regular_scl_def by blast
 
   show ?thesis
@@ -203,29 +619,34 @@ proof -
     case None
     hence "state_conflict S = None"
       by (simp add: S_def)
-    
-    have ball_N_not_empty: "\<forall>C \<in> N. C \<noteq> {#}" sorry
 
-    have "satisfiable (grounding_of_clss N)"
-      using trail_interp_clss_if_sound_and_trail_true[OF ]
-      (* using sound_S[unfolded S_def None] *)
-      apply (rule exI[where x = "trail_interp \<Gamma>"])
-      unfolding true_clss_def true_cls_def grounding_of_clss_def grounding_of_cls_def
-      unfolding imp_ex ball_UN ball_simps
-            
-      unfolding sound_state_def
-      sorry
-    moreover have "\<exists>\<gamma>. trail_true_clss \<Gamma> (N \<cdot>cs \<gamma>)"
-      using no_more_regular_step
-      unfolding S_def[unfolded None]
-      unfolding regular_scl_def
-      sorry
-    ultimately show ?thesis
-      unfolding S_def[unfolded None] state_trail_def state_conflict_def prod.sel
-      by simp
+    show ?thesis
+      using no_reasonable_decide
+    proof (elim disjE exE conjE)
+      assume "\<nexists>S'. decide N \<beta> S S'"
+      with no_new_conflict no_new_propagate
+      have "satisfiable {C \<in> grounding_of_clss N. multp (\<prec>\<^sub>B) C {#\<beta>#}} \<and>
+        trail_true_clss (state_trail S) {C \<in> grounding_of_clss N. multp (\<prec>\<^sub>B) C {#\<beta>#}}"
+        sorry
+      thus ?thesis ..
+    next
+      fix S' S''
+      assume "decide N \<beta> S S'" and "conflict N \<beta> S' S''"
+      hence "\<exists>S\<^sub>4. propagate N \<beta> S S\<^sub>4"
+        by (rule propagate_if_conflict_follows_decide[OF fin_N fin_learned_S no_new_conflict])
+      with no_new_propagate have False
+        by blast
+      thus ?thesis ..
+    qed
   next
     case (Some Cl)
     then obtain C \<gamma> where u_def: "u = Some (C, \<gamma>)" by force
+
+    have disj_vars_conflict: "\<forall>D \<in> N \<union> U \<union> clss_of_trail \<Gamma>. disjoint_vars C D" sorry
+    have domain_\<gamma>: "subst_domain \<gamma> \<subseteq> vars_cls C"
+      using conflict_min_subst_dom
+      by (simp add: S_def conflict_minimal_subst_domain_def u_def)
+
     show ?thesis
     proof (cases "C = {#}")
       case True
@@ -233,23 +654,101 @@ proof -
         using S_def u_def not_satisfiable_if_sound_state_conflict_bottom[OF sound_S] by simp
       thus ?thesis by simp
     next
-      case False
-      then obtain L C' where C_def: "C = C' + {#L#}"
-        by (metis add_mset_add_single multi_nonempty_split)
+      case C_not_empty: False
+      show ?thesis
+      proof (cases \<Gamma>)
+        case Nil
+        hence "C = {#}"
+          using S_def u_def
+          sorry
+        then show ?thesis
+          sorry
+      next
+        case (Cons Ln \<Gamma>')
+        then obtain L n where \<Gamma>_def: "\<Gamma> = (L, n) # \<Gamma>'"
+          by fastforce
+        show ?thesis
+        proof (cases "- L \<in># C \<cdot> \<gamma>")
+          case True \<comment> \<open>Literal cannot be skipped\<close>
+          show ?thesis
+          proof (cases n)
+            case None
+            then show ?thesis
+              sorry
+          next
+            case Some \<comment> \<open>Literal can be resolved\<close>
+            then obtain D L' \<sigma> where n_def: "n = Some (D, L', \<sigma>)"
+              by (metis prod_cases3)
+            with trail_propagate_wf have L_def: "L = L' \<cdot>l \<sigma>"
+              by (simp add: \<Gamma>_def S_def trail_propagated_wf_def)
+            hence 1: "\<Gamma> = trail_propagate \<Gamma>' L' D \<sigma> "
+              using \<Gamma>_def n_def
+              by (simp add: trail_propagate_def)
 
-      from no_more_regular_step have "\<nexists>S'. (reasonable_scl N)\<^sup>+\<^sup>+ (\<Gamma>, U, Some (C' + {#L#}, \<gamma>)) S'"
-        unfolding S_def u_def C_def
-        unfolding regular_scl_def
-        sorry
+            have domain_\<sigma>: "subst_domain \<sigma> \<subseteq> vars_cls (add_mset L' D)"
+              using trail_min_subst_dom
+              by (simp add: S_def trail_minimal_subst_domains_def 1 trail_propagate_def)
+            have ground_L'_D_\<sigma>: "is_ground_cls (add_mset L' D \<cdot> \<sigma>)"
+              using trail_groundings
+              by (simp add: S_def trail_groundings_def 1 trail_propagate_def)
 
-      then have False
-        unfolding reasonable_scl_def
-        sorry
+            obtain C' K where C_def: "C = C' + {#K#}" and K_\<gamma>: "K \<cdot>l \<gamma> = - L' \<cdot>l \<sigma>"
+              using True[unfolded L_def]
+              by (metis Melem_subst_cls add.right_neutral multi_member_split subst_minus
+                  union_mset_add_mset_right)
 
-      then show ?thesis by simp
+            define \<rho> :: "'v \<Rightarrow> ('f, 'v) Term.term" where
+              "\<rho> = renaming_wrt (N \<union> U \<union> clss_of_trail \<Gamma> \<union> {C' + {#K#}})"
+
+            have *: "vars_cls (add_mset L' D) \<inter> vars_cls (add_mset K C') = {}"
+              using disj_vars_conflict[unfolded C_def 1]
+              by (simp add: disjoint_vars_iff_inter_empty inf.commute)
+
+            have 2: "L' \<cdot>l \<sigma> = - (K \<cdot>l \<gamma>)"
+              using K_\<gamma> by fastforce
+            hence "atm_of L' \<cdot>a \<sigma> = atm_of K \<cdot>a \<gamma>"
+              by (metis atm_of_subst_lit atm_of_uminus)
+            hence "atm_of L' \<cdot>a (\<sigma> \<odot> \<gamma>) = atm_of K \<cdot>a (\<sigma> \<odot> \<gamma>)"
+              unfolding subst_subst_compose
+            proof (rule subst_subst_eq_subst_subst_if_subst_eq_substI(1))
+              show "vars_lit L' \<inter> subst_domain \<gamma> = {}"
+                using * domain_\<gamma> disj_vars_conflict
+                by (auto simp: C_def)
+            next
+              show "vars_lit K \<inter> subst_domain \<sigma> = {}"
+                using * domain_\<sigma> disj_vars_conflict by auto
+            next
+              have "range_vars \<sigma> = {}"
+                by (rule range_vars_eq_empty_if_is_ground[OF ground_L'_D_\<sigma> domain_\<sigma>])
+              thus "range_vars \<sigma> \<inter> subst_domain \<gamma> = {}"
+                by simp
+            qed
+            then obtain \<mu> where "Unification.mgu (atm_of L') (atm_of K) = Some \<mu>"
+              using ex_mgu_if_subst_eq_subst by blast
+            hence 3: "is_mimgu \<mu> {{atm_of L', atm_of K}}"
+              by (rule is_mimgu_if_mgu_eq_Some)
+
+            have "resolve N \<beta> (\<Gamma>, U, Some (C' + {#K#}, \<gamma>)) (\<Gamma>, U, Some ((C' + D) \<cdot> \<mu> \<cdot> \<rho>,
+              restrict_subst (vars_cls ((C' + D) \<cdot> \<mu> \<cdot> \<rho>)) (inv_renaming' \<rho> \<odot> \<gamma> \<odot> \<sigma>)))"
+              by (rule resolveI[OF 1 \<rho>_def 2 3])
+            with no_more_regular_step have False
+              unfolding regular_scl_def reasonable_scl_def scl_def
+              using S_def \<Gamma>_def C_def decide_well_defined(5) u_def by blast
+            thus ?thesis ..
+          qed
+        next
+          case False \<comment> \<open>Literal can be skipped\<close>
+          hence "skip N \<beta> ((L, n) # \<Gamma>', U, Some (C, \<gamma>)) (\<Gamma>', U, Some (C, \<gamma>))"
+            by (rule skipI[of L C \<gamma> N \<beta> n \<Gamma>' U])
+          with no_more_regular_step have False
+            using S_def \<Gamma>_def scl_def reasonable_scl_def regular_scl_def skip_well_defined(2) u_def
+            by blast
+          thus ?thesis ..
+        qed
+      qed
     qed
   qed
-  oops
+qed
 
 end
 
